src/syntax/FStar.Syntax.Embeddings.fsti
@@ -16,101 +16,19 @@
 
 module FStar.Syntax.Embeddings
 
-open FStar open FStar.Compiler
+open FStar
+open FStar.Compiler
 open FStar.Pervasives
 open FStar.Compiler.Effect
 open FStar.Syntax.Syntax
 open FStar.Char
 open FStar.VConfig
 
+include FStar.Syntax.Embeddings.Base
+
 module Range = FStar.Compiler.Range
 module Z = FStar.BigInt
 module BU = FStar.Compiler.Util
-
-(* TODO: Find a better home for these *)
-type norm_step =
-    | Simpl
-    | Weak
-    | HNF
-    | Primops
-    | Delta
-    | Zeta
-    | ZetaFull
-    | Iota
-    | Reify
-    | UnfoldOnly  of list string
-    | UnfoldFully of list string
-    | UnfoldAttr  of list string
-    | UnfoldQual  of list string
-    | UnfoldNamespace of list string    
-    | Unascribe
-    | NBE
-    | Unmeta
-
-type norm_cb = either Ident.lident term -> term // a callback to the normalizer
-
-type shadow_term = option (Thunk.t term)
-
-type embed_t = FStar.Compiler.Range.range -> shadow_term -> norm_cb -> term
-type unembed_t 'a = bool -> norm_cb -> option 'a // bool = whether we should warn on a failure
-
-type raw_embedder 'a   = 'a -> embed_t
-type raw_unembedder 'a = term -> unembed_t 'a
-
-val steps_Simpl         : term
-val steps_Weak          : term
-val steps_HNF           : term
-val steps_Primops       : term
-val steps_Delta         : term
-val steps_Zeta          : term
-val steps_ZetaFull      : term
-val steps_Iota          : term
-val steps_Reify         : term
-val steps_UnfoldOnly    : term
-val steps_UnfoldFully   : term
-val steps_UnfoldAttr    : term
-val steps_Unascribe     : term
-val steps_NBE           : term
-val steps_Unmeta        : term
-
-(*
- * Unmbedding functions return an option because they might fail
- * to interpret the given term as valid data. The `try_` version will
- * simply return None in that case, but the unsafe one will also raise a
- * warning, and should be used only where we really expect to always be
- * able to unembed.
- *)
-
-val id_norm_cb : norm_cb
-exception Embedding_failure
-exception Unembedding_failure
-
-val embedding (a:Type0) : Type0
-val emb_typ_of: embedding 'a -> emb_typ
-val term_as_fv: term -> fv //partial!
-val mk_emb : raw_embedder 'a -> raw_unembedder 'a -> fv -> embedding 'a
-val mk_emb_full: raw_embedder 'a
-              -> raw_unembedder 'a
-              -> typ
-              -> ('a -> string)
-              -> emb_typ
-              -> embedding 'a
-
-
-// embed: turning a value into a term (compiler internals -> userland)
-// unembed: interpreting a term as a value, which can fail (userland -> compiler internals)
-val embed        : embedding 'a -> 'a -> embed_t
-val unembed      : embedding 'a -> term -> unembed_t 'a
-val warn_unembed : embedding 'a -> term -> norm_cb -> option 'a
-val try_unembed  : embedding 'a -> term -> norm_cb -> option 'a
-val type_of      : embedding 'a -> typ
-val set_type     : typ -> embedding 'a -> embedding 'a
-
-val embed_as     : embedding 'a ->
-                   ('a -> 'b) ->
-                   ('b -> 'a) ->
-                   option typ -> (* optionally change the type *)
-                   embedding 'b
 
 (* Embeddings, both ways and containing type information *)
 val e_any         : embedding term // an identity
@@ -120,10 +38,8 @@ val e_char        : embedding char
 val e_int         : embedding Z.t
 val e_fsint       : embedding int
 val e_string      : embedding string
-val e_norm_step   : embedding norm_step
-val e_range       : embedding Range.range
+val e_norm_step   : embedding Pervasives.norm_step
 val e_vconfig     : embedding vconfig
-val e_issue       : embedding FStar.Errors.issue
 
 val e_option      : embedding 'a -> embedding (option 'a)
 val e_list        : embedding 'a -> embedding (list 'a)
@@ -133,6 +49,10 @@ val e_either      : embedding 'a -> embedding 'b -> embedding (either 'a 'b)
 val e_string_list : embedding (list string)
 val e_arrow       : embedding 'a -> embedding 'b -> embedding ('a -> 'b)
 val e_sealed      : embedding 'a -> embedding 'a
+
+val e___range     : embedding Range.range (* unsealed *)
+val e_range       : embedding Range.range (* sealed *)
+val e_issue       : embedding FStar.Errors.issue
 
 val mk_any_emb : typ -> embedding term
 
