src/extraction/FStar.Extraction.ML.RegEmb.fsti
@@ -1,0 +1,43 @@
+
+(*
+   Copyright 2008-2015 Abhishek Anand, Nikhil Swamy and Microsoft Research
+
+   Licensed under the Apache License, Version 2.0 (the "License");
+   you may not use this file except in compliance with the License.
+   You may obtain a copy of the License at
+
+       http://www.apache.org/licenses/LICENSE-2.0
+
+   Unless required by applicable law or agreed to in writing, software
+   distributed under the License is distributed on an "AS IS" BASIS,
+   WITHOUT WARRANTIES OR CONDITIONS OF ANY KIND, either express or implied.
+   See the License for the specific language governing permissions and
+   limitations under the License.
+*)
+module FStar.Extraction.ML.RegEmb
+
+(* This module handles registering plugins and generating
+embeddings for their types. *)
+
+open FStar
+open FStar.Compiler
+open FStar.Compiler.Effect
+
+open FStar.Syntax.Syntax
+open FStar.Extraction.ML
+open FStar.Extraction.ML.Syntax
+open FStar.Extraction.ML.UEnv
+
+(* When extracting a plugin, each top-level definition marked with a `@plugin` attribute
+   is extracted along with an invocation to FStar.Tactics.Native.register_tactic or register_plugin,
+   which installs the compiled term as a primitive step in the normalizer
+ *)
+val maybe_register_plugin (g:uenv) (se:sigelt) : list mlmodule1
+
+val interpret_plugin_as_term_fun :
+              UEnv.uenv
+            -> fv:fv
+            -> t:typ
+            -> arity:option int
+            -> ml_fv:mlexpr'
+            -> option (mlexpr * mlexpr * int * bool)
