src/extraction/FStar.Extraction.ML.Util.fsti
@@ -60,11 +60,3 @@ val mlloc_of_range : r:Range.range -> int * string
 val doms_and_cod : t:mlty -> list mlty * mlty
 val argTypes : t:mlty -> list mlty
 val uncurry_mlty_fun : t:mlty -> list mlty * mlty
-
-val interpret_plugin_as_term_fun :
-              UEnv.uenv
-            -> fv:S.fv
-            -> t:S.typ
-            -> arity:option int
-            -> ml_fv:mlexpr'
-            -> option (mlexpr * mlexpr * int * bool)
