src/parser/FStar.Parser.Const.fst
@@ -296,7 +296,8 @@ let hide   = p2l ["FStar"; "Ghost"; "hide"]
 
 (* FStar.Range *)
 let labeled_lid    = p2l ["FStar"; "Range"; "labeled"]
-let range_lid      = p2l ["FStar"; "Range"; "range"]
+let __range_lid    = p2l ["FStar"; "Range"; "__range"]
+let range_lid      = p2l ["FStar"; "Range"; "range"] (* this is a sealed version of the above *)
 let range_0        = p2l ["FStar"; "Range"; "range_0"]
 
 let guard_free     = pconst "guard_free"
