src/syntax/FStar.Syntax.Embeddings.Base.fst
@@ -1,0 +1,298 @@
+﻿(*
+   Copyright 2008-2014 Microsoft Research
+
+   Licensed under the Apache License, Version 2.0 (the "License");
+   you may not use this file except in compliance with the License.
+   You may obtain a copy of the License at
+
+       http://www.apache.org/licenses/LICENSE-2.0
+
+   Unless required by applicable law or agreed to in writing, software
+   distributed under the License is distributed on an "AS IS" BASIS,
+   WITHOUT WARRANTIES OR CONDITIONS OF ANY KIND, either express or implied.
+   See the License for the specific language governing permissions and
+   limitations under the License.
+*)
+
+module FStar.Syntax.Embeddings.Base
+
+open FStar
+open FStar.Compiler
+open FStar.Compiler.Effect
+open FStar.Compiler.Range
+open FStar.Pervasives
+open FStar.Syntax.Syntax
+
+module BU    = FStar.Compiler.Util
+module Err   = FStar.Errors
+module Ident = FStar.Ident
+module PC    = FStar.Parser.Const
+module Print = FStar.Syntax.Print
+module S     = FStar.Syntax.Syntax
+module SS    = FStar.Syntax.Subst
+module U     = FStar.Syntax.Util
+
+(*********************************************************************
+
+             A NOTE ON FUNCTIONS AND SHADOW TERMS
+
+Shadow terms exist to acomodate strong reduction of plugins.
+
+Suppose we have this function, marked as a plugin to accelerate it
+during typechecking:
+
+    [@@plugin]
+    let sort (l : list int) : list int = ...
+
+(Plugins are usually tactics, but do not have to be. This discussion
+is actually not so relevant for tactics as they do not run in open
+contexts.)
+
+Compilation will generate a version that works on _real_ concrete
+lists of integers. To call it on a term, as we have to do during
+typechecking, we need to wrap it with embeddings:
+
+    sort_term t = embed_intlist (sort (unembed_intlist t))
+
+This turns the term `t` into an actual `list int`, calls the native
+sort function, and then reconstructs a term for the resulting list.
+
+After loading the compiled version of that file, `sort_term` is now
+loaded as a primitive step in the normalizer (under the name `sort`, of
+course), and will be called everytime we find this symbol applied to an
+argument. While its argument must have already been reduced (CBV), there
+is no guarantee that it is an actual _value_ as we may be in an open
+context, e.g. we may be typechecking this formula:
+
+    forall l. sum (sort l) == sum l
+
+or it can be applied to some abstract lid even in a closed
+context, or to a Tm_let that we are not currently reducing (e.g. DIV),
+etc. So, we may fail (and often do) to unembed the argument term
+to obtain a concrete list, hence sort_term is closer to:
+
+    sort_term t = match unembed_intlist t with
+                  | None -> None
+                  | Some l -> embed_intlist (sort l)
+
+But, instead of stopping reduction with the None, we can instead
+use the definition of sort itself, and call the normalizer with
+the unfolded definition applied to the symbolic argument. Shadow
+terms are term representations of whatever the embedded thing is,
+which can be defaulted to when the embedding does not work.
+
+(TODO: what does this do for recursive functions? sounds
+  like it would not unfold? Actually, it seems broken:
+
+    [@@plugin]
+    let rec mylen (l : list int) : int =
+      match l with
+      | [] -> 0
+      | x::xs -> 1 + mylen xs
+
+    let test (a b c : int) =
+      assert (mylen [a;b;c] == mylen [c;b;a]) by begin
+        dump "1";
+        compute ();
+        dump "2";
+        trefl ();
+        ()
+      end
+
+this file works when mylen is not loaded as a plugin, but fails
+otherwise since reduction is blocked.)
+
+
+*********************************************************************)
+
+let id_norm_cb : norm_cb = function
+    | Inr x -> x
+    | Inl l -> S.fv_to_tm (S.lid_as_fv l None)
+exception Embedding_failure
+exception Unembedding_failure
+
+let map_shadow (s:shadow_term) (f:term -> term) : shadow_term =
+    BU.map_opt s (Thunk.map f)
+let force_shadow (s:shadow_term) = BU.map_opt s Thunk.force
+
+type embedding (a:Type0) = {
+  em : a -> embed_t;
+  un : term -> unembed_t a;
+  typ : typ;
+  print: printer a;
+  emb_typ: emb_typ
+}
+let emb_typ_of e = e.emb_typ
+
+let unknown_printer typ _ =
+    BU.format1 "unknown %s" (Print.term_to_string typ)
+
+let term_as_fv t =
+    match (SS.compress t).n with
+    | Tm_fvar fv -> fv
+    | _ -> failwith (BU.format1 "Embeddings not defined for type %s" (Print.term_to_string t))
+
+let mk_emb em un fv =
+    let typ = S.fv_to_tm fv in
+    {
+        em = em ;
+        un = un ;
+        typ = typ;
+        print=unknown_printer typ;
+        emb_typ=ET_app (S.lid_of_fv fv |> Ident.string_of_lid, [])
+    }
+
+let mk_emb_full em un typ printer emb_typ = {
+    em = em ;
+    un = un ;
+    typ = typ;
+    print = printer;
+    emb_typ = emb_typ
+}
+
+//
+// AR/NS: 04/22/2022:
+//        In the case of metaprograms, we reduce divergent terms in
+//        the normalizer, therefore, the final result that we get
+//        may be wrapped in a Meta_monadic node (e.g. lift, app, etc.)
+//        Before unembedding the result of such a computation,
+//          we strip those meta nodes
+//        In case the term inside is not a result, unembedding would
+//          anyway fail
+//        And we strip down only DIV
+//        Can we get any other effect? Not today, since from the client
+//          code, we enforce terms to be normalized to be PURE
+//
+
+let rec unmeta_div_results t =
+  let open FStar.Ident in
+  match (SS.compress t).n with
+  | Tm_meta {tm=t'; meta=Meta_monadic_lift (src, dst, _)} ->
+    if lid_equals src PC.effect_PURE_lid &&
+       lid_equals dst PC.effect_DIV_lid
+    then unmeta_div_results t'
+    else t
+
+  | Tm_meta {tm=t'; meta=Meta_monadic (m, _)} ->
+    if lid_equals m PC.effect_DIV_lid
+    then unmeta_div_results t'
+    else t
+
+  | Tm_meta {tm=t'} -> unmeta_div_results t'
+
+  | Tm_ascribed {tm=t'} -> unmeta_div_results t'
+
+  | _ -> t
+
+let type_of      (e:embedding 'a) = e.typ
+let printer_of   (e:embedding 'a) = e.print
+let set_type ty  (e:embedding 'a) = { e with typ = ty }
+
+let embed        (e:embedding 'a) = e.em
+let try_unembed  (e:embedding 'a) t n =
+  (* Unembed always receives a term without the meta_monadics above,
+  strip it here. TODO: maybe also compress? *)
+  let t = unmeta_div_results t in
+  e.un t n
+
+let unembed (e:embedding 'a) t n =
+  let r = try_unembed e t n in
+  if None? r then
+    Err.log_issue t.pos (Err.Warning_NotEmbedded,
+              BU.format3 "Warning, unembedding failed for type %s (%s); term = %s"
+                          (Print.term_to_string (type_of e))
+                          (Print.emb_typ_to_string (emb_typ_of e))
+                          (Print.term_to_string t)
+                          );
+  r
+
+
+let embed_as (ea:embedding 'a) (ab : 'a -> 'b) (ba : 'b -> 'a) (o:option typ) =
+    mk_emb_full (fun (x:'b) -> embed ea (ba x))
+                (fun (t:term) cb -> BU.map_opt (try_unembed ea t cb) ab)
+                (match o with | Some t -> t | _ -> type_of ea)
+                (fun (x:'b) -> BU.format1 "(embed_as>> %s)\n" (ea.print (ba x)))
+                ea.emb_typ
+
+(* A simple lazy embedding, without cancellations nor an expressive type. *)
+let e_lazy #a (k:lazy_kind) (ty : typ) : embedding a =
+  let ee (x:a) rng _topt _norm : term = U.mk_lazy x ty k (Some rng) in
+  let uu (t:term) _norm : option a =
+    let t0 = t in
+    match (SS.compress t).n with
+    | Tm_lazy {blob=b; lkind=lkind} when U.eq_lazy_kind lkind k -> Some (Dyn.undyn b)
+    | Tm_lazy {blob=b; lkind=lkind} ->
+      (* This is very likely a bug, warn! *)
+      Err.log_issue t0.pos (Err.Warning_NotEmbedded,
+                BU.format3 "Warning, lazy unembedding failed, tag mismatch.\n\t\
+                            Expected %s, got %s\n\t\
+                            t = %s."
+                            (U.lazy_kind_to_string lkind) (U.lazy_kind_to_string k)
+                            (Print.term_to_string t0));
+      None
+    | _ ->
+      None
+  in
+  mk_emb ee uu (term_as_fv ty)
+
+let lazy_embed (pa:printer 'a) (et:emb_typ) rng ta (x:'a) (f:unit -> term) =
+    if !Options.debug_embedding
+    then BU.print3 "Embedding a %s\n\temb_typ=%s\n\tvalue is %s\n"
+                         (Print.term_to_string ta)
+                         (Print.emb_typ_to_string et)
+                         (pa x);
+    if !Options.eager_embedding
+    then f()
+    else let thunk = Thunk.mk f in
+         U.mk_lazy x S.tun (Lazy_embedding (et, thunk)) (Some rng)
+
+let lazy_unembed (pa:printer 'a) (et:emb_typ) (x:term) (ta:term) (f:term -> option 'a) : option 'a =
+    let x = SS.compress x in
+    match x.n with
+    | Tm_lazy {blob=b; lkind=Lazy_embedding (et', t)}  ->
+      if et <> et'
+      || !Options.eager_embedding
+      then let res = f (Thunk.force t) in
+           let _ = if !Options.debug_embedding
+                   then BU.print3 "Unembed cancellation failed\n\t%s <> %s\nvalue is %s\n"
+                                (Print.emb_typ_to_string et)
+                                (Print.emb_typ_to_string et')
+                                (match res with None -> "None" | Some x -> "Some " ^ (pa x))
+           in
+           res
+      else let a = Dyn.undyn b in
+           let _ = if !Options.debug_embedding
+                   then BU.print2 "Unembed cancelled for %s\n\tvalue is %s\n"
+                                (Print.emb_typ_to_string et)
+                                  (pa a)
+           in
+           Some a
+    | _ ->
+      let aopt = f x in
+      let _ = if !Options.debug_embedding
+              then BU.print3 "Unembedding:\n\temb_typ=%s\n\tterm is %s\n\tvalue is %s\n"
+                               (Print.emb_typ_to_string et)
+                               (Print.term_to_string x)
+                               (match aopt with None -> "None" | Some a -> "Some " ^ pa a) in
+      aopt
+
+let (let?) o f = BU.bind_opt o f
+
+let mk_extracted_embedding (name: string) (u: string & list term -> option 'a) (e: 'a -> term) : embedding 'a =
+  let uu (t:term) _norm : option 'a =
+    let hd, args = U.head_and_args t in
+    let? hd_lid =
+      match (SS.compress (U.un_uinst hd)).n with
+      | Tm_fvar fv -> Some fv.fv_name.v
+      | _ -> None
+    in
+    u (Ident.string_of_lid hd_lid, List.map fst args)
+  in
+  let ee (x:'a) rng _topt _norm : term = e x in
+  mk_emb ee uu (S.lid_as_fv (Ident.lid_of_str name) None)
+
+let extracted_embed (e: embedding 'a) (x: 'a) : term =
+  embed e x Range.dummyRange None id_norm_cb
+
+let extracted_unembed (e: embedding 'a) (t: term) : option 'a =
+  try_unembed e t id_norm_cb
