src/syntax/FStar.Syntax.Syntax.fsti
@@ -409,6 +409,7 @@ and lazy_kind =
   | Lazy_universe
   | Lazy_universe_uvar
   | Lazy_issue
+  | Lazy_ident
 and binding =
   | Binding_var      of bv
   | Binding_lid      of lident * (univ_names * typ)
@@ -846,6 +847,7 @@ val t_real          : term
 val t_float         : term
 val t_char          : term
 val t_range         : term
+val t___range       : term
 val t_vconfig       : term
 val t_norm_step     : term
 val t_term          : term
