src/typechecker/FStar.TypeChecker.Cfg.fsti
@@ -156,4 +156,4 @@ val config: list step -> Env.env -> cfg
 
 val should_reduce_local_let : cfg -> letbinding -> bool
 
-val translate_norm_steps: list EMB.norm_step -> list Env.step
+val translate_norm_steps: list Pervasives.norm_step -> list Env.step
